

Questions with Answer Keys

MathonGo

Q1 (20 July 2021 Shift 1)

If the value of $\lim_{x \rightarrow 0} (2 - \cos x \sqrt{\cos 2x}) \left(\frac{x+2}{x^2} \right)$ is equal to e^n , then n is equal to _____

Q2 (20 July 2021 Shift 2)

If $f : \mathbf{R} \rightarrow \mathbf{R}$ is given by $f(x) = x + 1$, then the value of

$$\lim_{n \rightarrow \infty} \frac{1}{n} \left[f(0) + f\left(\frac{5}{n}\right) + f\left(\frac{10}{n}\right) + \dots + f\left(\frac{5(n-1)}{n}\right) \right]$$

is:

(1) $\frac{3}{2}$

(2) $\frac{5}{2}$

(3) $\frac{1}{2}$

(4) $\frac{7}{2}$

Q3 (20 July 2021 Shift 2)

If $\lim_{x \rightarrow 0} \frac{\alpha x e^x - \beta \log_e(1+x) + \gamma x^2 e^{-x}}{x \sin^2 x} = 10$, $\alpha, \beta, \gamma \in \mathbf{R}$, then the value of $\alpha + \beta + \gamma$ is

Q4 (27 July 2021 Shift 1)

Let $f : \mathbf{R} \rightarrow \mathbf{R}$ be a function such that $f(2) = 4$ and $f'(2) = 1$. Then, the value of $\lim_{x \rightarrow 2} \frac{x^2 f(2) - 4f(x)}{x-2}$ is equal to :

(1) 4

(2) 8

(3) 16

(4) 12

Q5 (27 July 2021 Shift 2)

The value of $\lim_{x \rightarrow 0} \left(\frac{x}{\sqrt[3]{1-\sin x} - \sqrt[3]{1+\sin x}} \right)$ is equal

to:

(1) 0

MathonGo

(4) -1

mathongo mathongo #MathBoleToMathGya mathongo mathongo

Hints and Solutions

MathonGo

Q1

$$\lim_{x \rightarrow 0} (2 - \cos x \sqrt{\cos x})^{\frac{x+2}{x^2}}$$

form: 1^∞

$$= e^{\lim_{x \rightarrow 0} \left(\frac{1 - \cos x \sqrt{\cos 2x}}{x^2} \right) \times (x+2)}$$

$$\text{Now } \lim_{x \rightarrow 0} \frac{1 - \cos x \sqrt{\cos 2x}}{x^2}$$

$$= \lim_{x \rightarrow 0} \frac{\sin x \sqrt{\cos 2x} - \cos x \times \frac{1}{2\sqrt{\cos 2x}} \times (-2 \sin 2x)}{2x}$$

(by L' Hospital Rule)

$$\lim_{x \rightarrow 0} \frac{\sin x \cos 2x + \sin 2x \cdot \cos x}{2x}$$

$$= \frac{1}{2} + 1 = \frac{3}{2}$$

$$\text{So, } e^{\lim_{x \rightarrow 0} \left(\frac{1 - \cos x \sqrt{\cos 2x}}{x^2} \right) (x+2)}$$

$$= e^{\frac{3}{2} \times 2} = e^3$$

$$\Rightarrow a = 3$$

Q2

$$I = \sum_{r=0}^{n-1} f\left(\frac{5r}{n}\right) \frac{1}{n}$$

$$I = \int_0^1 f(5x) dx$$

$$I = \int_0^1 (5x + 1) dx$$

$$I = \left[\frac{5x^2}{2} + x \right]_0^1$$

$$I = \frac{5}{2} + 1 = \frac{7}{2}$$

Q3

$$\lim_{x \rightarrow 0} \frac{\alpha x \left(1 + x + \frac{x^2}{2}\right) - \beta \left(x - \frac{x^2}{2} + \frac{x^3}{3}\right) + \gamma x^2 (1 - x)}{x^3}$$

$$\lim_{x \rightarrow 0} \frac{x(\alpha - \beta) + x^2 \left(\alpha + \frac{\beta}{2} + \gamma\right) + x^3 \left(\frac{\alpha}{2} - \frac{\beta}{3} - \gamma\right)}{x^3} = 10$$

For limit to exist

$$\alpha - \beta = 0, \alpha + \frac{\beta}{2} + \gamma = 0$$

$$\frac{\alpha}{2} - \frac{\beta}{3} - \gamma = 10$$

Hints and Solutions

MathonGo

$$\beta = \alpha, \gamma = -3\frac{\alpha}{2}$$

Put in (i)

$$\frac{\alpha}{2} - \frac{\alpha}{3} + \frac{3\alpha}{2} = 10$$

$$\frac{\alpha}{6} + \frac{3\alpha}{2} = 10 \Rightarrow \frac{\alpha+9\alpha}{6} = 10$$

$$\Rightarrow \alpha = 6$$

$$\alpha = 6, \beta = 6, \gamma = -9$$

$$\alpha + \beta + \gamma = 3$$

Q4

$$\text{Apply L'Hopital Rule } \lim_{x \rightarrow 2} \left(\frac{2xf(2) - 4f'(x)}{1} \right)$$

$$= \frac{4(4) - 4}{1} = 12$$

Q5

$$\lim_{x \rightarrow 0} \left(\frac{x}{\sqrt[8]{1-\sin x} - \sqrt[8]{1+\sin x}} \right)$$

$$= \lim_{x \rightarrow 0} \left(\frac{x}{\sqrt[8]{1-\sin x} - \sqrt[8]{1+\sin x}} \right)$$

$$= \lim_{x \rightarrow 0} \left(\frac{x}{\sqrt[8]{1-\sin x} - \sqrt[8]{1+\sin x}} \right)$$

$$\left(\frac{\sqrt[8]{1-\sin x} + \sqrt[8]{1+\sin x}}{\sqrt[8]{1-\sin x} + \sqrt[8]{1+\sin x}} \right)$$

$$\left(\frac{\sqrt[4]{1-\sin x} + \sqrt[4]{1+\sin x}}{\sqrt[4]{1-\sin x} + \sqrt[4]{1+\sin x}} \right)$$

$$\left(\frac{\sqrt[2]{1-\sin x} + \sqrt[2]{1+\sin x}}{\sqrt[2]{1-\sin x} + \sqrt[2]{1+\sin x}} \right)$$

$$= \lim_{x \rightarrow 0} \left(\frac{x}{1 - \sin x - (1 + \sin x)} \right)$$

$$(\sqrt[8]{1-\sin x} + \sqrt[8]{1+\sin x})(\sqrt[4]{1-\sin x} + \sqrt[4]{1+\sin x})$$

$$(\sqrt[2]{1-\sin x} + \sqrt[2]{1+\sin x})$$

$$= \lim_{x \rightarrow 0} \frac{x}{(-2\sin x)} (\sqrt[8]{1-\sin x} + \sqrt[8]{1+\sin x})$$

$$(\sqrt[4]{1-\sin x} + \sqrt[4]{1+\sin x})(\sqrt[2]{1-\sin x} + \sqrt[2]{1+\sin x})$$

$$= \lim_{x \rightarrow 0} \left(-\frac{1}{2} \right) (2) (2) (2) \left\{ \because \lim_{x \rightarrow 0} \frac{\sin x}{x} = 1 \right\} = -4$$